Array: write_ok

src/Array.v
@@ -4,6 +4,15 @@ Require Import List Omega Ring Word Pred Prog Hoare SepAuto BasicProg.
 Notation "$" := (natToWord _).
 Ltac words := ring_prepare; ring.
 
+Lemma pimpl_or : forall p q p' q',
+  p ==> p'
+  -> q ==> q'
+  -> p \/ q ==> p' \/ q'.
+Proof.
+  firstorder.
+Qed.
+
+
 (** * A generic array predicate: a sequence of consecutive points-to facts *)
 
 Fixpoint array (a : addr) (vs : list valu) :=
@@ -26,6 +35,102 @@ Fixpoint selN (vs : list valu) (n : nat) : valu :=
 
 Definition sel (vs : list valu) (i : addr) : valu :=
   selN vs (wordToNat i).
+
+Fixpoint updN (vs : list valu) (n : nat) (v : valu) : list valu :=
+  match vs with
+    | nil => nil
+    | v' :: vs' =>
+      match n with
+        | O => v :: vs'
+        | S n' => v' :: updN vs' n' v
+      end
+  end.
+
+Definition upd (vs : list valu) (i : addr) (v : valu) : list valu :=
+  updN vs (wordToNat i) v.
+
+Lemma length_updN : forall vs n v, length (updN vs n v) = length vs.
+Proof.
+  induction vs; destruct n; simpl; intuition.
+Qed.
+
+Theorem length_upd : forall vs i v, length (upd vs i v) = length vs.
+Proof.
+  intros; apply length_updN.
+Qed.
+
+Hint Rewrite length_updN length_upd.
+
+Lemma selN_updN_eq : forall vs n v,
+  n < length vs
+  -> selN (updN vs n v) n = v.
+Proof.
+  induction vs; destruct n; simpl; intuition; omega.
+Qed.
+
+Lemma sel_upd_eq : forall vs i v,
+  wordToNat i < length vs
+  -> sel (upd vs i v) i = v.
+Proof.
+  intros; apply selN_updN_eq; auto.
+Qed.
+
+Hint Rewrite selN_updN_eq sel_upd_eq using omega.
+
+Lemma firstn_updN : forall v vs i j,
+  i <= j
+  -> firstn i (updN vs j v) = firstn i vs.
+Proof.
+  induction vs; destruct i, j; simpl; intuition.
+  omega.
+  rewrite IHvs; auto; omega.
+Qed.
+
+Lemma firstn_upd : forall v vs i j,
+  i <= wordToNat j
+  -> firstn i (upd vs j v) = firstn i vs.
+Proof.
+  intros; apply firstn_updN; auto.
+Qed.
+
+Hint Rewrite firstn_updN firstn_upd using omega.
+
+Lemma skipN_updN' : forall v vs i j,
+  i > j
+  -> skipn i (updN vs j v) = skipn i vs.
+Proof.
+  induction vs; destruct i, j; simpl; intuition; omega.
+Qed.
+
+Lemma skipn_updN : forall v vs i j,
+  i >= j
+  -> match updN vs j v with
+       | nil => nil
+       | _ :: vs' => skipn i vs'
+     end
+     = match vs with
+         | nil => nil
+         | _ :: vs' => skipn i vs'
+       end.
+Proof.
+  destruct vs, j; simpl; eauto using skipN_updN'.
+Qed.
+
+Lemma skipn_upd : forall v vs i j,
+  i >= wordToNat j
+  -> match upd vs j v with
+       | nil => nil
+       | _ :: vs' => skipn i vs'
+     end
+     = match vs with
+         | nil => nil
+         | _ :: vs' => skipn i vs'
+       end.
+Proof.
+  intros; apply skipn_updN; auto.
+Qed.
+
+Hint Rewrite skipn_updN skipn_upd using omega.
 
 
 (** * Isolating an array cell *)
@@ -108,12 +213,22 @@ Qed.
 Module Type ARRAY_OPS.
   Parameter ArrayRead : addr -> addr -> (valu -> prog) -> prog.
   Axiom ArrayRead_eq : ArrayRead = fun a i k => Read (a ^+ i) k.
+
+  Parameter ArrayWrite : addr -> addr -> valu -> (unit -> prog) -> prog.
+  Axiom ArrayWrite_eq : ArrayWrite = fun a i v k => Write (a ^+ i) v k.
 End ARRAY_OPS.
 
 Module ArrayOps : ARRAY_OPS.
   Definition ArrayRead : addr -> addr -> (valu -> prog) -> prog :=
     fun a i k => Read (a ^+ i) k.
   Theorem ArrayRead_eq : ArrayRead = fun a i k => Read (a ^+ i) k.
+  Proof.
+    auto.
+  Qed.
+
+  Definition ArrayWrite : addr -> addr -> valu -> (unit -> prog) -> prog :=
+    fun a i v k => Write (a ^+ i) v k.    
+  Theorem ArrayWrite_eq : ArrayWrite = fun a i v k => Write (a ^+ i) v k.
   Proof.
     auto.
   Qed.
@@ -168,5 +283,67 @@ Proof.
   eapply pimpl_ok; [ eassumption | cancel ].
   eapply pimpl_trans; [ | apply pimpl_sep_star; [ apply pimpl_refl
                                                 | apply isolate_bwd; eassumption ] ].
+  cancel.
+Qed.
+
+Theorem write_ok:
+  forall (a i:addr) (v:valu) (rx:unit->prog) (rec:prog),
+  {{ exists vs F, array a vs * F
+   * [[wordToNat i < length vs]]
+   * [[{{ array a (upd vs i v) * F }} (rx tt) >> rec]]
+   * [[{{ array a vs * F \/ array a (upd vs i v) * F }} rec >> rec]]
+  }} ArrayWrite a i v rx >> rec.
+Proof.
+  intros.
+  apply pimpl_ok with (exists vs F,
+    array a (firstn (wordToNat i) vs)
+    * (a ^+ i) |-> sel vs i
+    * array (a ^+ i ^+ $1) (skipn (S (wordToNat i)) vs) * F
+    * [[wordToNat i < length vs]]
+    * [[{{ array a (firstn (wordToNat i) vs)
+           * (a ^+ i) |-> v
+           * array (a ^+ i ^+ $1) (skipn (S (wordToNat i)) vs) * F }} (rx tt) >> rec]]
+    * [[{{ (array a (firstn (wordToNat i) vs)
+           * (a ^+ i) |-> sel vs i
+           * array (a ^+ i ^+ $1) (skipn (S (wordToNat i)) vs) * F)
+           \/ (array a (firstn (wordToNat i) vs)
+           * (a ^+ i) |-> v
+           * array (a ^+ i ^+ $1) (skipn (S (wordToNat i)) vs) * F) }} rec >> rec]])%pred.
+
+  rewrite ArrayWrite_eq.
+  eapply pimpl_ok.
+  apply write_ok.
+  cancel.
+  eapply pimpl_ok; [ eassumption | cancel ].
+  eapply pimpl_ok; [ eassumption | cancel ].
+
+  cancel.
+  eapply pimpl_trans; [ apply pimpl_sep_star; [ apply pimpl_refl
+                                              | apply pimpl_sep_star; [ apply pimpl_refl
+                                                                      | apply isolate_fwd; eassumption ] ] | ].
+  cancel.
+  assumption.
+
+  eapply pimpl_ok; [ eassumption | cancel ].
+  eapply pimpl_trans; [ | apply pimpl_sep_star; [ apply pimpl_refl
+                                                | apply isolate_bwd; autorewrite with core; eassumption ] ].
+  autorewrite with core.
+  cancel.
+  autorewrite with core.
+  cancel.
+
+  eapply pimpl_ok; [ eassumption | apply pimpl_or; cancel ].
+  eapply pimpl_trans; [ | apply pimpl_sep_star; [ apply pimpl_refl
+                                                | apply isolate_bwd; autorewrite with core; eassumption ] ].
+  autorewrite with core.
+  cancel.
+  autorewrite with core.
+  cancel.
+
+  eapply pimpl_trans; [ | apply pimpl_sep_star; [ apply pimpl_refl
+                                                | apply isolate_bwd; autorewrite with core; eassumption ] ].
+  autorewrite with core.
+  cancel.
+  autorewrite with core.
   cancel.
 Qed.
